src/examples/crash_lock.v
@@ -1,0 +1,369 @@
+From iris.bi Require Import lib.fractional.
+From iris.proofmode Require Import tactics.
+
+From Perennial.program_logic Require Import staged_invariant.
+
+From self.base Require Import primitive_laws.
+From self.lang Require Import lang.
+From self.high Require Import dprop.
+
+From self.lang Require Import notation lang.
+From self.algebra Require Import view.
+From self.base Require Import primitive_laws class_instances crash_borrow.
+From self.high Require Import proofmode wpc_proofmode if_rec.
+From self.high Require Import dprop abstract_state_instances modalities
+     resources crash_weakestpre weakestpre crash_borrow weakestpre_na weakestpre_at
+     recovery_weakestpre lifted_modalities protocol protocols no_buffer
+     mapsto_na_flushed.
+From self.high.modalities Require Import fence.
+
+From self.examples Require Import spin_lock.
+
+Section crash_lock.
+  Context `{!nvmG Σ, lockG Σ, stagedG Σ} (Nlock : namespace).
+
+  (* Definition is_free_crash_lock lk : iProp Σ := *)
+  (*   is_free_lock lk ∗ pre_borrow. *)
+
+  Definition is_crash_lock γ (lk : val) (R Rc : dProp Σ) `{!ViewObjective Rc} : dProp Σ :=
+    is_lock Nlock γ lk (crash_borrow R Rc).
+
+  Definition crash_locked γ lk R Rcrash `{!ViewObjective Rcrash} : dProp Σ :=
+    (crash_borrow R Rcrash ∗
+     is_lock Nlock γ lk (crash_borrow R Rcrash) ∗
+     locked γ)%I.
+
+  (* Definition partial_crash_locked lk R Rcrash `{!ViewObjective Rcrash} : dProp Σ := *)
+  (*   (∃ R' Rcrash', *)
+  (*    □ (R' -∗ Rcrash') ∗ *)
+  (*    □ (Rcrash' -∗ Rcrash ∗ (Rcrash -∗ Rcrash')) ∗ *)
+  (*    crash_borrow R Rcrash ∗ *)
+  (*    crash_borrow ((R -∗ R') ∧ (Rcrash -∗ Rcrash')) (Rcrash -∗ Rcrash') ∗ *)
+  (*    is_lock Nlock lk (crash_borrow R' Rcrash') ∗ *)
+  (*    locked lk)%I. *)
+
+  (* Lemma wp_new_free_crash_lock : *)
+  (*   {{{ True }}} lock.new #() {{{ lk, RET #lk; is_free_crash_lock lk }}}. *)
+  (* Proof. *)
+  (*   iIntros (Φ) "_ HΦ". *)
+  (*   iApply (wpc_wp _ O). *)
+  (*   iApply wpc_crash_borrow_generate_pre; auto. *)
+  (*   iApply wp_wpc. *)
+  (*   wp_apply wp_new_free_lock. *)
+  (*   iIntros. iApply "HΦ". iFrame. *)
+  (* Qed. *)
+
+  Lemma wpc_crash_borrow_init_ctx' s e Φ Φc P Pc `{!ViewObjective Pc} K `{!LanguageCtx K} :
+    to_val e = None →
+    P -∗
+    □ (P -∗ Pc) -∗
+    Φc ∧ (crash_borrow P Pc -∗
+          WPC e @ s; (⊤ ∖ (↑borrowN : coPset))
+                  {{ λ v, WPC K (of_val v) @ s; ⊤ {{ Φ }} {{ Φc }} }}
+                  {{ Φc }}) -∗
+    WPC K e @ s; ⊤ {{ Φ }} {{ Φc ∗ Pc }}.
+  Proof.
+  Admitted.
+
+  Lemma wp_wpc_frame' s E1 e Φ Φc `{!ViewObjective Φc} R :
+    (Φc ∧ R) ∗
+    WP e @ s; E1 {{ λ v, R -∗ Φ v }} ⊢
+    WPC e @ s; E1 {{ Φ }} {{ Φc }}.
+  Proof.
+    iIntros "(HΦc&Hwp)".
+    iApply (wpc_strong_mono' s s E1 E1 _ (λ v, R ∗ (R -∗ Φ v))%I _ (Φc ∗ True)%I
+          with "[-]"); auto.
+  Admitted.
+  (*   { iApply wpc_frame_l'. *)
+  (*     rewrite comm; iFrame. *)
+  (*     iApply wp_wpc; eauto. } *)
+  (*   iSplit. *)
+  (*   - iIntros (?). rewrite wand_elim_r. iIntros; eauto. *)
+  (*   - iIntros "(H&?)". iApply (fupd_mask_intro_discard); eauto. *)
+  (* Qed. *)
+
+  Global Instance crash_borrow_buffer_free R Rc `{BufferFree R, BufferFree Rc}
+      `{!ViewObjective Rc} :
+    BufferFree (crash_borrow R Rc).
+  Proof.
+    rewrite /IntoNoBuffer.
+    iModel. destruct TV as [[SV PV] BF]. simpl.
+    iIntros "[#H bor]".
+    rewrite !monPred_at_intuitionistically.
+    monPred_simpl.
+    iSplitL "".
+    { iModIntro. introsIndex [[??]?] ?.
+      iSpecialize ("H" $! (_, _, BF, gnames)).
+      rewrite 4!buffer_free_at.
+      iApply "H".
+      iPureIntro. split; last done. solve_view_le. }
+    iApply crash_borrow_proper; last iApply "bor".
+    rewrite (buffer_free_at R).
+    done.
+  Qed.
+
+  Lemma newlock_crash_spec k (R Rcrash : dProp Σ)
+      K `{!LanguageCtx K} Φ (Φc : dProp Σ)
+      `{!ViewObjective Rcrash, !ViewObjective Φc}
+      `{!BufferFree R, !BufferFree Rcrash} :
+    R -∗
+    □ (R -∗ Rcrash) -∗
+    Φc ∧ (∀ lk γ, is_crash_lock γ lk R Rcrash -∗
+    WPC (K (of_val lk)) @ k; ⊤ {{ Φ }} {{ Φc }}) -∗
+    WPC K (mk_lock #()) @ k; ⊤ {{ Φ }} {{ Φc ∗ Rcrash }}.
+  Proof.
+    iIntros "HR #Hwand1 Hwpc".
+    iApply (wpc_crash_borrow_init_ctx' _ _ _ _ R Rcrash with "[$] [$] [-]").
+    { auto. }
+    iSplit.
+    { iDestruct "Hwpc" as "($&_)". }
+    iIntros "Hborrow".
+    iApply (wp_wpc_frame').
+    iSplitL "Hwpc".
+    { iExact "Hwpc". }
+    iApply (mk_lock_spec Nlock (crash_borrow R Rcrash) with "[$Hborrow]").
+    iNext.
+    iIntros (? lk) "His_lock HP".
+    iApply "HP". eauto.
+  Qed.
+
+  (*
+  Lemma alloc_crash_lock k Φ Φc e lk (R Rcrash : dProp Σ):
+    □ (R -∗ Rcrash) ∗
+    R ∗
+    is_free_crash_lock lk ∗
+    (is_crash_lock #lk R Rcrash -∗
+          WPC e @ k; ⊤ {{ Φ }} {{ Rcrash -∗ Φc }}) -∗
+    WPC e @ k; ⊤ {{ Φ }} {{ Φc }}.
+  Proof.
+    clear.
+    iIntros "(#HRcrash&HR&Hfree&Hwp)".
+    iDestruct "Hfree" as "(Hfree1&Htoks)".
+    iApply (wpc_crash_borrow_inits with "[$] HR HRcrash").
+    iIntros "Hborrow".
+    iMod (alloc_lock with "[$] [Hborrow]") as "H".
+    { iNext. iExact "Hborrow". }
+    iApply "Hwp". iFrame.
+  Qed.
+  *)
+
+  Lemma acquire_crash_spec γ E (R Rcrash : dProp Σ)
+    `{BufferFree R, BufferFree Rcrash, !ViewObjective Rcrash} lk :
+    ↑Nlock ⊆ E →
+    {{{ is_crash_lock γ lk R Rcrash }}}
+    acquire lk @ E
+    {{{ RET #(); crash_locked γ lk R Rcrash }}}.
+  Proof.
+    iIntros (? Φ) "#Hcrash HΦ".
+    wp_apply (acquire_spec with "Hcrash"); auto.
+    iIntros "(? & ?)". iApply "HΦ". iFrame. iFrame "#".
+  Qed.
+
+  (*
+  Lemma partial_try_acquire_spec E lk R Rcrash R' Rcrash':
+    ↑Nlock ⊆ E →
+    □ (R' -∗ R ∗ (R -∗ R') ∧ (Rcrash -∗ Rcrash')) -∗
+    □ (R -∗ Rcrash) -∗
+    □ (Rcrash' -∗ Rcrash ∗ (Rcrash -∗ Rcrash')) -∗
+    {{{ is_crash_lock lk R' Rcrash' }}} lock.try_acquire lk @ E
+    {{{ b, RET #b; if b is true then partial_crash_locked lk R Rcrash else True }}}.
+  Proof.
+    iIntros (?) "#Hw1 #Hw2 #Hw3".
+    iIntros (Φ) "!> Hl HΦ".
+    rewrite /is_crash_lock/is_lock.
+    iDestruct "Hl" as (l ->) "#Hinv".
+    wp_rec. wp_bind (CmpXchg _ _ _). iInv Nlock as ([]) "[Hl HR]".
+    - wp_cmpxchg_fail. iModIntro. iSplitL "Hl"; first (iNext; iExists true; eauto).
+      wp_pures. iApply ("HΦ" $! false). done.
+    - iDestruct "HR" as "[Hl2 HR]".
+      iCombine "Hl Hl2" as "Hl".
+      rewrite Qp_quarter_three_quarter.
+      iApply (wpc_wp NotStuck 0 _ _ _ True).
+      iAssert (▷ □ (R' -∗ Rcrash'))%I with "[HR]" as "#Hwand".
+      { iNext. by iApply crash_borrow_crash_wand. }
+      iApply (wpc_crash_borrow_split _ _ _ _ _ _ _
+                                     R
+                                     ((R -∗ R') ∧ (Rcrash -∗ Rcrash'))
+                                     Rcrash
+                                     (Rcrash -∗ Rcrash')
+                with "HR"); auto.
+      { iNext. iModIntro. iIntros "H". iDestruct "H" as "(_&$)". }
+      { iNext. iIntros "(HR1&HR2)". iApply "HR2"; eauto. }
+      iApply wp_wpc.
+      wp_cmpxchg_suc.
+      iModIntro.
+      iEval (rewrite -Qp_quarter_three_quarter) in "Hl".
+      iDestruct (fractional.fractional_split_1 with "Hl") as "[Hl1 Hl2]".
+      iIntros "(Hc1&Hc2)".
+      iSplit; first done. iModIntro.
+      iSplitL "Hl1".
+      { iNext; iExists true; eauto. }
+      wp_pures. iApply "HΦ". iModIntro.
+      rewrite /partial_crash_locked.
+      iExists _, _. iFrame "∗ #".
+      rewrite /is_lock/locked.
+      iSplitL ""; eauto.
+  Qed.
+
+  Lemma partial_acquire_spec E lk R Rcrash R' Rcrash':
+    ↑Nlock ⊆ E →
+    □ (R' -∗ R ∗ (R -∗ R') ∧ (Rcrash -∗ Rcrash')) -∗
+    □ (R -∗ Rcrash) -∗
+    □ (Rcrash' -∗ Rcrash ∗ (Rcrash -∗ Rcrash')) -∗
+    {{{ is_crash_lock lk R' Rcrash' }}} lock.acquire lk @ E {{{ RET #(); partial_crash_locked lk R Rcrash }}}.
+  Proof.
+    iIntros (?) "#H1 #H2 #H3". iIntros (Φ) "!> #Hl HΦ". iLöb as "IH". wp_rec.
+    iPoseProof (partial_try_acquire_spec E with "H1 H2") as "H"; first done.
+    wp_apply "H"; auto.
+    iIntros ([]).
+    - iIntros "Hlked". wp_if. iApply "HΦ"; by iFrame.
+    - iIntros "_". wp_if. iApply ("IH" with "[HΦ]"). auto.
+  Qed.
+*)
+
+  Lemma use_crash_locked γ E1 e lk R Rcrash Φ Φc
+                         `{!ViewObjective Rcrash, !ViewObjective Φc} :
+    to_val e = None →
+    crash_locked γ lk R Rcrash -∗
+    Φc ∧ (R -∗ WPC e @ E1 {{ λ v, (crash_locked γ lk R Rcrash -∗ (Φc ∧ Φ v)) ∗ R }}
+                                         {{ Φc ∗ Rcrash }}) -∗
+    WPC e @ E1 {{ Φ }} {{ Φc }}.
+  Proof.
+    iIntros (?) "Hcrash_locked H".
+    iDestruct "Hcrash_locked" as "(Hfull & #His_lock & Hlocked)".
+    iApply (wpc_crash_borrow_open with "[$]"); auto.
+    iSplit.
+    - iDestruct "H" as "($&_)".
+    - iIntros "HR". iDestruct "H" as "(_&H)".
+      iSpecialize ("H" with "[$]").
+      iApply (wpc_strong_mono with "H"); eauto.
+      iSplit.
+      * iIntros (?) "(Hclose&?)". iModIntro. iFrame. iFrame "#".
+        iIntros. iApply "Hclose". iFrame; eauto.
+      * iIntros.  iIntros "!>". eauto.
+  Qed.
+
+  Lemma release_spec γ E (R Rcrash : dProp Σ)
+    `{BufferFree R} `{!ViewObjective Rcrash} lk :
+    ↑Nlock ⊆ E →
+    {{{ crash_locked γ lk R Rcrash }}}
+    release lk @ E
+    {{{ RET #(); True }}}.
+  Proof.
+    iIntros (? Φ) "Hcrash_locked HΦ".
+    iDestruct "Hcrash_locked" as "(Hfull&#His_lock&Hlocked)".
+  Admitted.
+  (*   wp_apply (release_spec' with "[His_lock Hlocked Hfull]"); swap 1 2. *)
+  (*   { iFrame "His_lock". iFrame. } *)
+  (*   { auto. } *)
+  (*   by iApply "HΦ". *)
+  (* Qed. *)
+
+  (*
+  Lemma partial_release_spec E (R Rcrash : dProp Σ) lk:
+    ↑Nlock ⊆ E →
+    {{{ partial_crash_locked lk R Rcrash }}}
+    lock.release lk @ E
+    {{{ RET #(); True }}}.
+  Proof.
+    iIntros (? Φ) "Hcrash_locked HΦ".
+    iDestruct "Hcrash_locked" as (??) "(#Hw1&#Hw2&Hc1&Hc2&His_lock&Hlocked)".
+    rewrite /is_lock.
+    iDestruct "His_lock" as (l ->) "#Hinv".
+    rewrite /lock.release /=. wp_lam.
+    wp_bind (CmpXchg _ _ _).
+    iInv Nlock as (b) "[>Hl _]".
+
+    iDestruct (locked_loc with "Hlocked") as "Hl2".
+    iDestruct (heap_mapsto_agree with "[$Hl $Hl2]") as %->.
+    iCombine "Hl Hl2" as "Hl".
+    rewrite Qp_quarter_three_quarter.
+    iApply (wpc_wp NotStuck 0 _ _ _ True).
+    iApply (wpc_crash_borrow_combine _ _ _ _ _ R' Rcrash'
+                  with "Hc1 Hc2"); auto.
+    { iNext. iIntros "(HR&Hw)". iDestruct "Hw" as "(H&_)". iApply "H". eauto. }
+    iApply wp_wpc.
+    wp_cmpxchg_suc.
+    iModIntro.
+    iIntros "Hb". iSplit; first done.
+    iModIntro.
+    iSplitR "HΦ"; last by wp_seq; iApply "HΦ".
+    iEval (rewrite -Qp_quarter_three_quarter) in "Hl".
+    iDestruct (fractional.fractional_split_1 with "Hl") as "[Hl1 Hl2]".
+    iNext. iExists false. iFrame.
+  Qed.
+*)
+
+  Definition with_lock lk e :=
+    (acquire lk;;
+     let: "v" := e in
+     release lk)%E.
+
+  Lemma wpc_frame (s : stuckness) (E1 : coPset)
+          (e: expr) (Φ Φ': val -> dProp Σ) (Φc Φc': dProp Σ) (R : dPropI Σ) :
+      R -∗
+      WPC e @ s; E1 {{ v, Φ v }} {{Φc}} -∗
+      (R ∗ Φc -∗ Φc') -∗
+      (∀ v, R ∗ Φ v -∗ Φ' v) -∗
+      WPC e @ s; E1 {{ v, Φ' v }} {{Φc'}}.
+  Proof.
+    iIntros "F Hwpc HΦc' HΦ'".
+  Admitted.
+  (*   iDestruct (wpc_frame_l with "[F $Hwpc]") as "Hwpc". *)
+  (*   { iExact "F". } *)
+  (*   iApply (wpc_strong_mono' with "Hwpc"); eauto. *)
+  (*   iSplit. *)
+  (*   - iIntros (v) "HΦ". *)
+  (*     iApply ("HΦ'" with "HΦ"). *)
+  (*   - iIntros "HΦc". *)
+  (*     iApply fupd_mask_intro_discard; [ set_solver+ | ]. *)
+  (*     iApply ("HΦc'" with "HΦc"). *)
+  (* Qed. *)
+
+  Lemma with_lock_spec γ Φ Φc (R Rcrash : dProp Σ) lk e
+                         `{!ViewObjective Rcrash, !ViewObjective Φc} :
+    to_val e = None →
+    is_crash_lock γ lk R Rcrash ∗
+    (Φc ∧ (R -∗ WPC e @ ⊤ {{ λ v, (Φc ∧ Φ #()) ∗ R }} {{ Φc ∗ Rcrash }})) -∗
+    WPC (with_lock lk e) @ ⊤ {{ Φ }} {{ Φc }}.
+  Proof.
+    iIntros (Hnv) "(#Hcrash&Hwp)".
+    rewrite /with_lock.
+    wpc_bind (acquire lk).
+  Admitted.
+  (*
+    wpc_frame "Hwp".
+    { iDestruct "Hwp" as "($&_)".  }
+    iApply (acquire_spec with "Hcrash").
+    { set_solver. }
+    iNext. iIntros "H Hwp".
+    wpc_pures.
+    { iDestruct "Hwp" as "($&_)". }
+
+    wpc_bind e.
+    iApply (use_crash_locked with "[$]"); eauto.
+    iSplit.
+    { iDestruct "Hwp" as "($&_)". }
+    iIntros "HR". iDestruct "Hwp" as "(_&H)".
+    iSpecialize ("H" with "[$]").
+    iApply (wpc_strong_mono with "H"); eauto.
+    iSplit; last first.
+    { iIntros. iModIntro. iFrame. }
+    iIntros (?) "(H&?)". iModIntro. iFrame.
+    iIntros "Hlocked".
+    iSplit.
+    { iDestruct "H" as "(H&_)". eauto. }
+
+    wpc_pures.
+    { iDestruct "H" as "(H&_)". eauto. }
+
+    wpc_frame "H".
+    { iDestruct "H" as "($&_)". }
+    iApply (release_spec with "Hlocked").
+    { auto. }
+    iNext. iIntros "_ H".
+    { iDestruct "H" as "(_&$)". }
+  Qed.
+*)
+
+End crash_lock.
